theories/L2k_noCnstrParams/wNorm.v
@@ -24,8 +24,8 @@ Variable p:environ Term.
 Inductive WNorm: Term -> Prop :=
 | WNLam: forall nm bod, WNorm (TLambda nm bod)
 | WNFix: forall ds br, WNorm (TFix ds br)
-| WNCase: forall mch brs,
-    WNorm mch -> ~ isCanonical mch -> WNorm (TCase mch brs)
+| WNCase: forall i mch brs,
+    WNorm mch -> ~ isCanonical mch -> WNorm (TCase i mch brs)
 | WNConstruct: forall i n arty, WNorm (TConstruct i n arty)
 | WNApp: forall fn t ts,
     WNorm fn -> WNorm t -> WNorms ts ->
